$r_0$ = 0.1, index = 0, nrun = 0: $$-1.40 \cdot 10^{+00} \cdot I - 8.95 \cdot 10^{+00} \cdot I^4 + 7.03 \cdot 10^{+00} \cdot I^2 - 2.05 \cdot 10^{-04} = \frac{dI}{dy}$$

$r_0$ = 0.1, index = 0, nrun = 1: $$-1.40 \cdot 10^{+00} \cdot I - 8.95 \cdot 10^{+00} \cdot I^4 + 7.03 \cdot 10^{+00} \cdot I^2 - 2.05 \cdot 10^{-04} = \frac{dI}{dy}$$

$r_0$ = 0.1, index = 0, nrun = 2: $$3.49 \cdot 10^{+00} \cdot I^2 + 1.61 \cdot 10^{-04} = \frac{dI}{dy}$$

$r_0$ = 0.1, index = 1, nrun = 0: $$-1.40 \cdot 10^{+00} \cdot I - 8.95 \cdot 10^{+00} \cdot I^4 + 7.03 \cdot 10^{+00} \cdot I^2 - 2.05 \cdot 10^{-04} = \frac{dI}{dy}$$

$r_0$ = 0.1, index = 1, nrun = 1: $$-8.68 \cdot 10^{-02} \cdot I + 1.33 \cdot 10^{+01} \cdot I^4 + 2.15 \cdot 10^{+01} \cdot I^2 + 8.53 \cdot 10^{-06} + 3.43 \cdot 10^{+01} \cdot I^3 = \frac{dI}{dy}$$

$r_0$ = 0.1, index = 1, nrun = 2: $$-1.40 \cdot 10^{+00} \cdot I - 8.95 \cdot 10^{+00} \cdot I^4 + 7.03 \cdot 10^{+00} \cdot I^2 - 2.05 \cdot 10^{-04} = \frac{dI}{dy}$$

$r_0$ = 0.1, index = 2, nrun = 0: $$-1.40 \cdot 10^{+00} \cdot I - 8.95 \cdot 10^{+00} \cdot I^4 + 7.03 \cdot 10^{+00} \cdot I^2 - 2.05 \cdot 10^{-04} = \frac{dI}{dy}$$

$r_0$ = 0.1, index = 2, nrun = 1: $$-1.40 \cdot 10^{+00} \cdot I - 8.95 \cdot 10^{+00} \cdot I^4 + 7.03 \cdot 10^{+00} \cdot I^2 - 2.05 \cdot 10^{-04} = \frac{dI}{dy}$$

$r_0$ = 0.1, index = 2, nrun = 2: $$-1.40 \cdot 10^{+00} \cdot I - 8.95 \cdot 10^{+00} \cdot I^4 + 7.03 \cdot 10^{+00} \cdot I^2 - 2.05 \cdot 10^{-04} = \frac{dI}{dy}$$

$r_0$ = 0.1, index = 3, nrun = 0: $$-1.40 \cdot 10^{+00} \cdot I - 8.95 \cdot 10^{+00} \cdot I^4 + 7.03 \cdot 10^{+00} \cdot I^2 - 2.05 \cdot 10^{-04} = \frac{dI}{dy}$$

$r_0$ = 0.1, index = 3, nrun = 1: $$-1.40 \cdot 10^{+00} \cdot I - 8.95 \cdot 10^{+00} \cdot I^4 + 7.03 \cdot 10^{+00} \cdot I^2 - 2.05 \cdot 10^{-04} = \frac{dI}{dy}$$

$r_0$ = 0.1, index = 3, nrun = 2: $$3.49 \cdot 10^{+00} \cdot I^2 + 1.61 \cdot 10^{-04} = \frac{dI}{dy}$$

$r_0$ = 0.1, index = 4, nrun = 0: $$3.49 \cdot 10^{+00} \cdot I^2 + 1.61 \cdot 10^{-04} = \frac{dI}{dy}$$

$r_0$ = 0.1, index = 4, nrun = 1: $$3.49 \cdot 10^{+00} \cdot I^2 + 1.61 \cdot 10^{-04} = \frac{dI}{dy}$$

$r_0$ = 0.1, index = 4, nrun = 2: $$-1.40 \cdot 10^{+00} \cdot I - 8.95 \cdot 10^{+00} \cdot I^4 + 7.03 \cdot 10^{+00} \cdot I^2 - 2.05 \cdot 10^{-04} = \frac{dI}{dy}$$

$r_0$ = 0.1, index = 5, nrun = 0: $$3.49 \cdot 10^{+00} \cdot I^2 + 1.61 \cdot 10^{-04} = \frac{dI}{dy}$$

$r_0$ = 0.2, index = 0, nrun = 0: $$-1.98 \cdot 10^{+00} \cdot I - 1.45 \cdot 10^{-03} = \frac{dI}{dy}$$

$r_0$ = 0.2, index = 0, nrun = 1: $$-6.80 \cdot 10^{-01} \cdot I + 9.19 \cdot 10^{+00} \cdot I^2 - 4.72 \cdot 10^{-04} + 9.20 \cdot 10^{+00} \cdot I^3 = \frac{dI}{dy}$$

$r_0$ = 0.2, index = 0, nrun = 2: $$-1.98 \cdot 10^{+00} \cdot I - 1.45 \cdot 10^{-03} = \frac{dI}{dy}$$

$r_0$ = 0.2, index = 1, nrun = 0: $$-1.98 \cdot 10^{+00} \cdot I - 1.45 \cdot 10^{-03} = \frac{dI}{dy}$$

$r_0$ = 0.2, index = 1, nrun = 1: $$-1.98 \cdot 10^{+00} \cdot I - 1.45 \cdot 10^{-03} = \frac{dI}{dy}$$

$r_0$ = 0.2, index = 1, nrun = 2: $$-1.98 \cdot 10^{+00} \cdot I - 1.45 \cdot 10^{-03} = \frac{dI}{dy}$$

$r_0$ = 0.2, index = 2, nrun = 0: $$-1.98 \cdot 10^{+00} \cdot I - 1.45 \cdot 10^{-03} = \frac{dI}{dy}$$

$r_0$ = 0.2, index = 2, nrun = 1: $$-1.98 \cdot 10^{+00} \cdot I - 1.45 \cdot 10^{-03} = \frac{dI}{dy}$$

$r_0$ = 0.2, index = 2, nrun = 2: $$-1.98 \cdot 10^{+00} \cdot I - 1.45 \cdot 10^{-03} = \frac{dI}{dy}$$

$r_0$ = 0.2, index = 3, nrun = 0: $$-1.98 \cdot 10^{+00} \cdot I - 1.45 \cdot 10^{-03} = \frac{dI}{dy}$$

$r_0$ = 0.2, index = 3, nrun = 1: $$-1.98 \cdot 10^{+00} \cdot I - 1.45 \cdot 10^{-03} = \frac{dI}{dy}$$

$r_0$ = 0.2, index = 3, nrun = 2: $$-1.98 \cdot 10^{+00} \cdot I - 1.45 \cdot 10^{-03} = \frac{dI}{dy}$$

$r_0$ = 0.2, index = 4, nrun = 0: $$-6.80 \cdot 10^{-01} \cdot I + 9.19 \cdot 10^{+00} \cdot I^2 - 4.72 \cdot 10^{-04} + 9.20 \cdot 10^{+00} \cdot I^3 = \frac{dI}{dy}$$

$r_0$ = 0.2, index = 4, nrun = 1: $$-6.80 \cdot 10^{-01} \cdot I + 9.19 \cdot 10^{+00} \cdot I^2 - 4.72 \cdot 10^{-04} + 9.20 \cdot 10^{+00} \cdot I^3 = \frac{dI}{dy}$$

$r_0$ = 0.2, index = 4, nrun = 2: $$-6.80 \cdot 10^{-01} \cdot I + 9.19 \cdot 10^{+00} \cdot I^2 - 4.72 \cdot 10^{-04} + 9.20 \cdot 10^{+00} \cdot I^3 = \frac{dI}{dy}$$

$r_0$ = 0.2, index = 5, nrun = 1: $$7.07 \cdot 10^{-01} \cdot I + 3.04 \cdot 10^{+01} \cdot I^4 + 2.86 \cdot 10^{+01} \cdot I^2 + 4.95 \cdot 10^{-04} + 5.65 \cdot 10^{+01} \cdot I^3 = \frac{dI}{dy}$$

$r_0$ = 0.2, index = 5, nrun = 2: $$7.07 \cdot 10^{-01} \cdot I + 3.04 \cdot 10^{+01} \cdot I^4 + 2.86 \cdot 10^{+01} \cdot I^2 + 4.95 \cdot 10^{-04} + 5.65 \cdot 10^{+01} \cdot I^3 = \frac{dI}{dy}$$

$r_0$ = 0.3, index = 0, nrun = 0: $$-6.99 \cdot 10^{-01} \cdot I + 1.10 \cdot 10^{+00} \cdot I^2 - 5.85 \cdot 10^{-04} = \frac{dI}{dy}$$

$r_0$ = 0.3, index = 0, nrun = 1: $$2.18 \cdot 10^{+00} \cdot I^2 + 3.32 \cdot 10^{-04} = \frac{dI}{dy}$$

$r_0$ = 0.3, index = 0, nrun = 2: $$2.18 \cdot 10^{+00} \cdot I^2 + 3.32 \cdot 10^{-04} = \frac{dI}{dy}$$

$r_0$ = 0.3, index = 1, nrun = 0: $$2.18 \cdot 10^{+00} \cdot I^2 + 3.32 \cdot 10^{-04} = \frac{dI}{dy}$$

$r_0$ = 0.3, index = 1, nrun = 1: $$2.18 \cdot 10^{+00} \cdot I^2 + 3.32 \cdot 10^{-04} = \frac{dI}{dy}$$

$r_0$ = 0.3, index = 1, nrun = 2: $$2.18 \cdot 10^{+00} \cdot I^2 + 3.32 \cdot 10^{-04} = \frac{dI}{dy}$$

$r_0$ = 0.3, index = 2, nrun = 0: $$2.18 \cdot 10^{+00} \cdot I^2 + 3.32 \cdot 10^{-04} = \frac{dI}{dy}$$

$r_0$ = 0.3, index = 2, nrun = 1: $$2.18 \cdot 10^{+00} \cdot I^2 + 3.32 \cdot 10^{-04} = \frac{dI}{dy}$$

$r_0$ = 0.3, index = 2, nrun = 2: $$2.18 \cdot 10^{+00} \cdot I^2 + 3.32 \cdot 10^{-04} = \frac{dI}{dy}$$

$r_0$ = 0.3, index = 3, nrun = 0: $$-6.99 \cdot 10^{-01} \cdot I + 1.10 \cdot 10^{+00} \cdot I^2 - 5.85 \cdot 10^{-04} = \frac{dI}{dy}$$

$r_0$ = 0.3, index = 3, nrun = 1: $$-6.99 \cdot 10^{-01} \cdot I + 1.10 \cdot 10^{+00} \cdot I^2 - 5.85 \cdot 10^{-04} = \frac{dI}{dy}$$

$r_0$ = 0.3, index = 3, nrun = 2: $$-6.99 \cdot 10^{-01} \cdot I + 1.10 \cdot 10^{+00} \cdot I^2 - 5.85 \cdot 10^{-04} = \frac{dI}{dy}$$

$r_0$ = 0.3, index = 4, nrun = 0: $$-6.99 \cdot 10^{-01} \cdot I + 1.10 \cdot 10^{+00} \cdot I^2 - 5.85 \cdot 10^{-04} = \frac{dI}{dy}$$

$r_0$ = 0.3, index = 4, nrun = 1: $$-6.99 \cdot 10^{-01} \cdot I + 1.10 \cdot 10^{+00} \cdot I^2 - 5.85 \cdot 10^{-04} = \frac{dI}{dy}$$

$r_0$ = 0.3, index = 4, nrun = 2: $$-6.99 \cdot 10^{-01} \cdot I + 1.10 \cdot 10^{+00} \cdot I^2 - 5.85 \cdot 10^{-04} = \frac{dI}{dy}$$

$r_0$ = 0.3, index = 5, nrun = 0: $$-6.99 \cdot 10^{-01} \cdot I + 1.10 \cdot 10^{+00} \cdot I^2 - 5.85 \cdot 10^{-04} = \frac{dI}{dy}$$

$r_0$ = 0.3, index = 5, nrun = 1: $$-6.99 \cdot 10^{-01} \cdot I + 1.10 \cdot 10^{+00} \cdot I^2 - 5.85 \cdot 10^{-04} = \frac{dI}{dy}$$

$r_0$ = 0.3, index = 5, nrun = 2: $$-6.99 \cdot 10^{-01} \cdot I + 1.10 \cdot 10^{+00} \cdot I^2 - 5.85 \cdot 10^{-04} = \frac{dI}{dy}$$

$r_0$ = 0.4, index = 0, nrun = 0: $$-1.09 \cdot 10^{+00} \cdot I - 1.75 \cdot 10^{-03} = \frac{dI}{dy}$$

$r_0$ = 0.4, index = 0, nrun = 1: $$-1.09 \cdot 10^{+00} \cdot I - 1.75 \cdot 10^{-03} = \frac{dI}{dy}$$

$r_0$ = 0.4, index = 0, nrun = 2: $$-1.09 \cdot 10^{+00} \cdot I - 1.75 \cdot 10^{-03} = \frac{dI}{dy}$$

$r_0$ = 0.4, index = 1, nrun = 0: $$-1.09 \cdot 10^{+00} \cdot I - 1.75 \cdot 10^{-03} = \frac{dI}{dy}$$

$r_0$ = 0.4, index = 1, nrun = 1: $$-1.09 \cdot 10^{+00} \cdot I - 1.75 \cdot 10^{-03} = \frac{dI}{dy}$$

$r_0$ = 0.4, index = 1, nrun = 2: $$-1.09 \cdot 10^{+00} \cdot I - 1.75 \cdot 10^{-03} = \frac{dI}{dy}$$

$r_0$ = 0.4, index = 2, nrun = 0: $$-1.09 \cdot 10^{+00} \cdot I - 1.75 \cdot 10^{-03} = \frac{dI}{dy}$$

$r_0$ = 0.4, index = 2, nrun = 1: $$-1.09 \cdot 10^{+00} \cdot I - 1.75 \cdot 10^{-03} = \frac{dI}{dy}$$

$r_0$ = 0.4, index = 2, nrun = 2: $$-1.09 \cdot 10^{+00} \cdot I - 1.75 \cdot 10^{-03} = \frac{dI}{dy}$$

$r_0$ = 0.4, index = 3, nrun = 0: $$-1.09 \cdot 10^{+00} \cdot I - 1.75 \cdot 10^{-03} = \frac{dI}{dy}$$

$r_0$ = 0.4, index = 3, nrun = 1: $$-1.09 \cdot 10^{+00} \cdot I - 1.75 \cdot 10^{-03} = \frac{dI}{dy}$$

$r_0$ = 0.4, index = 3, nrun = 2: $$-1.09 \cdot 10^{+00} \cdot I - 1.75 \cdot 10^{-03} = \frac{dI}{dy}$$

$r_0$ = 0.4, index = 4, nrun = 0: $$-1.09 \cdot 10^{+00} \cdot I - 1.75 \cdot 10^{-03} = \frac{dI}{dy}$$

$r_0$ = 0.4, index = 5, nrun = 0: $$-1.09 \cdot 10^{+00} \cdot I - 1.75 \cdot 10^{-03} = \frac{dI}{dy}$$

$r_0$ = 0.5, index = 0, nrun = 0: $$-2.33 \cdot 10^{-01} \cdot I + 5.49 \cdot 10^{-01} \cdot I^2 - 5.07 \cdot 10^{-04} = \frac{dI}{dy}$$

$r_0$ = 0.5, index = 0, nrun = 1: $$-2.33 \cdot 10^{-01} \cdot I + 5.49 \cdot 10^{-01} \cdot I^2 - 5.07 \cdot 10^{-04} = \frac{dI}{dy}$$

$r_0$ = 0.5, index = 0, nrun = 2: $$-2.33 \cdot 10^{-01} \cdot I + 5.49 \cdot 10^{-01} \cdot I^2 - 5.07 \cdot 10^{-04} = \frac{dI}{dy}$$

$r_0$ = 0.5, index = 1, nrun = 0: $$-2.33 \cdot 10^{-01} \cdot I + 5.49 \cdot 10^{-01} \cdot I^2 - 5.07 \cdot 10^{-04} = \frac{dI}{dy}$$

$r_0$ = 0.5, index = 1, nrun = 1: $$-2.33 \cdot 10^{-01} \cdot I + 5.49 \cdot 10^{-01} \cdot I^2 - 5.07 \cdot 10^{-04} = \frac{dI}{dy}$$

$r_0$ = 0.5, index = 1, nrun = 2: $$-2.33 \cdot 10^{-01} \cdot I + 5.49 \cdot 10^{-01} \cdot I^2 - 5.07 \cdot 10^{-04} = \frac{dI}{dy}$$

$r_0$ = 0.5, index = 2, nrun = 0: $$-2.33 \cdot 10^{-01} \cdot I + 5.49 \cdot 10^{-01} \cdot I^2 - 5.07 \cdot 10^{-04} = \frac{dI}{dy}$$

$r_0$ = 0.5, index = 2, nrun = 1: $$-2.33 \cdot 10^{-01} \cdot I + 5.49 \cdot 10^{-01} \cdot I^2 - 5.07 \cdot 10^{-04} = \frac{dI}{dy}$$

$r_0$ = 0.5, index = 2, nrun = 2: $$-2.33 \cdot 10^{-01} \cdot I + 5.49 \cdot 10^{-01} \cdot I^2 - 5.07 \cdot 10^{-04} = \frac{dI}{dy}$$

$r_0$ = 0.5, index = 3, nrun = 0: $$-2.33 \cdot 10^{-01} \cdot I + 5.49 \cdot 10^{-01} \cdot I^2 - 5.07 \cdot 10^{-04} = \frac{dI}{dy}$$

$r_0$ = 0.5, index = 3, nrun = 1: $$-2.33 \cdot 10^{-01} \cdot I + 5.49 \cdot 10^{-01} \cdot I^2 - 5.07 \cdot 10^{-04} = \frac{dI}{dy}$$

$r_0$ = 0.5, index = 3, nrun = 2: $$-2.33 \cdot 10^{-01} \cdot I + 5.49 \cdot 10^{-01} \cdot I^2 - 5.07 \cdot 10^{-04} = \frac{dI}{dy}$$

$r_0$ = 0.5, index = 4, nrun = 0: $$-2.33 \cdot 10^{-01} \cdot I + 5.49 \cdot 10^{-01} \cdot I^2 - 5.07 \cdot 10^{-04} = \frac{dI}{dy}$$

$r_0$ = 0.5, index = 4, nrun = 1: $$-2.33 \cdot 10^{-01} \cdot I + 5.49 \cdot 10^{-01} \cdot I^2 - 5.07 \cdot 10^{-04} = \frac{dI}{dy}$$

$r_0$ = 0.5, index = 4, nrun = 2: $$-2.33 \cdot 10^{-01} \cdot I + 5.49 \cdot 10^{-01} \cdot I^2 - 5.07 \cdot 10^{-04} = \frac{dI}{dy}$$

$r_0$ = 0.5, index = 5, nrun = 0: $$-2.33 \cdot 10^{-01} \cdot I + 5.49 \cdot 10^{-01} \cdot I^2 - 5.07 \cdot 10^{-04} = \frac{dI}{dy}$$

$r_0$ = 0.5, index = 5, nrun = 1: $$-2.33 \cdot 10^{-01} \cdot I + 5.49 \cdot 10^{-01} \cdot I^2 - 5.07 \cdot 10^{-04} = \frac{dI}{dy}$$

$r_0$ = 0.5, index = 5, nrun = 2: $$-2.33 \cdot 10^{-01} \cdot I + 5.49 \cdot 10^{-01} \cdot I^2 - 5.07 \cdot 10^{-04} = \frac{dI}{dy}$$

$r_0$ = 0.6, index = 0, nrun = 0: $$-1.18 \cdot 10^{+00} \cdot I^4 + 1.53 \cdot 10^{+00} \cdot I^2 + 2.64 \cdot 10^{-04} = \frac{dI}{dy}$$

$r_0$ = 0.6, index = 0, nrun = 1: $$-1.59 \cdot 10^{-01} \cdot I - 4.50 \cdot 10^{+00} \cdot I^4 - 3.17 \cdot 10^{-01} \cdot I^2 - 4.68 \cdot 10^{-04} - 4.83 \cdot 10^{+00} \cdot I^3 = \frac{dI}{dy}$$

$r_0$ = 0.6, index = 0, nrun = 2: $$-1.18 \cdot 10^{+00} \cdot I^4 + 1.53 \cdot 10^{+00} \cdot I^2 + 2.64 \cdot 10^{-04} = \frac{dI}{dy}$$

$r_0$ = 0.6, index = 1, nrun = 0: $$-1.18 \cdot 10^{+00} \cdot I^4 + 1.53 \cdot 10^{+00} \cdot I^2 + 2.64 \cdot 10^{-04} = \frac{dI}{dy}$$

$r_0$ = 0.6, index = 1, nrun = 1: $$-1.18 \cdot 10^{+00} \cdot I^4 + 1.53 \cdot 10^{+00} \cdot I^2 + 2.64 \cdot 10^{-04} = \frac{dI}{dy}$$

$r_0$ = 0.6, index = 1, nrun = 2: $$-1.18 \cdot 10^{+00} \cdot I^4 + 1.53 \cdot 10^{+00} \cdot I^2 + 2.64 \cdot 10^{-04} = \frac{dI}{dy}$$

$r_0$ = 0.6, index = 2, nrun = 0: $$-1.59 \cdot 10^{-01} \cdot I - 4.50 \cdot 10^{+00} \cdot I^4 - 3.17 \cdot 10^{-01} \cdot I^2 - 4.68 \cdot 10^{-04} - 4.83 \cdot 10^{+00} \cdot I^3 = \frac{dI}{dy}$$

$r_0$ = 0.6, index = 2, nrun = 1: $$-1.18 \cdot 10^{+00} \cdot I^4 + 1.53 \cdot 10^{+00} \cdot I^2 + 2.64 \cdot 10^{-04} = \frac{dI}{dy}$$

$r_0$ = 0.6, index = 2, nrun = 2: $$-1.11 \cdot 10^{-01} \cdot I - 2.75 \cdot 10^{+00} \cdot I^4 - 2.01 \cdot 10^{-04} - 3.18 \cdot 10^{+00} \cdot I^3 - 2.19 \cdot 10^{-01} \cdot d^2I/dy^2 = \frac{dI}{dy}$$

$r_0$ = 0.6, index = 3, nrun = 0: $$-1.87 \cdot 10^{+01} \cdot I + 5.08 \cdot 10^{+01} \cdot I^2 - 7.86 \cdot 10^{-02} = \frac{dI}{dy}$$

$r_0$ = 0.6, index = 3, nrun = 1: $$-1.18 \cdot 10^{+00} \cdot I^4 + 1.53 \cdot 10^{+00} \cdot I^2 + 2.64 \cdot 10^{-04} = \frac{dI}{dy}$$

$r_0$ = 0.6, index = 3, nrun = 2: $$-1.18 \cdot 10^{+00} \cdot I^4 + 1.53 \cdot 10^{+00} \cdot I^2 + 2.64 \cdot 10^{-04} = \frac{dI}{dy}$$

$r_0$ = 0.7, index = 0, nrun = 0: $$-1.67 \cdot 10^{-01} \cdot I + 4.52 \cdot 10^{-01} \cdot I^2 - 6.93 \cdot 10^{-04} = \frac{dI}{dy}$$

$r_0$ = 0.7, index = 0, nrun = 1: $$-1.67 \cdot 10^{-01} \cdot I + 4.52 \cdot 10^{-01} \cdot I^2 - 6.93 \cdot 10^{-04} = \frac{dI}{dy}$$

$r_0$ = 0.7, index = 0, nrun = 2: $$-1.67 \cdot 10^{-01} \cdot I + 4.52 \cdot 10^{-01} \cdot I^2 - 6.93 \cdot 10^{-04} = \frac{dI}{dy}$$

$r_0$ = 0.7, index = 1, nrun = 0: $$-1.67 \cdot 10^{-01} \cdot I + 4.52 \cdot 10^{-01} \cdot I^2 - 6.93 \cdot 10^{-04} = \frac{dI}{dy}$$

$r_0$ = 0.7, index = 1, nrun = 1: $$-1.67 \cdot 10^{-01} \cdot I + 4.52 \cdot 10^{-01} \cdot I^2 - 6.93 \cdot 10^{-04} = \frac{dI}{dy}$$

$r_0$ = 0.7, index = 1, nrun = 2: $$-1.36 \cdot 10^{-01} \cdot I - 2.51 \cdot 10^{+00} \cdot I^4 - 3.72 \cdot 10^{-04} - 2.69 \cdot 10^{+00} \cdot I^3 = \frac{dI}{dy}$$

$r_0$ = 0.7, index = 2, nrun = 0: $$-1.67 \cdot 10^{-01} \cdot I + 4.52 \cdot 10^{-01} \cdot I^2 - 6.93 \cdot 10^{-04} = \frac{dI}{dy}$$

$r_0$ = 0.7, index = 2, nrun = 1: $$-1.67 \cdot 10^{-01} \cdot I + 4.52 \cdot 10^{-01} \cdot I^2 - 6.93 \cdot 10^{-04} = \frac{dI}{dy}$$

$r_0$ = 0.7, index = 2, nrun = 2: $$-1.67 \cdot 10^{-01} \cdot I + 4.52 \cdot 10^{-01} \cdot I^2 - 6.93 \cdot 10^{-04} = \frac{dI}{dy}$$

$r_0$ = 0.7, index = 3, nrun = 0: $$-1.67 \cdot 10^{-01} \cdot I + 4.52 \cdot 10^{-01} \cdot I^2 - 6.93 \cdot 10^{-04} = \frac{dI}{dy}$$

$r_0$ = 0.7, index = 3, nrun = 1: $$-1.67 \cdot 10^{-01} \cdot I + 4.52 \cdot 10^{-01} \cdot I^2 - 6.93 \cdot 10^{-04} = \frac{dI}{dy}$$

$r_0$ = 0.7, index = 3, nrun = 2: $$-1.67 \cdot 10^{-01} \cdot I + 4.52 \cdot 10^{-01} \cdot I^2 - 6.93 \cdot 10^{-04} = \frac{dI}{dy}$$

$r_0$ = 0.7, index = 4, nrun = 0: $$-1.67 \cdot 10^{-01} \cdot I + 4.52 \cdot 10^{-01} \cdot I^2 - 6.93 \cdot 10^{-04} = \frac{dI}{dy}$$

$r_0$ = 0.7, index = 4, nrun = 1: $$-1.67 \cdot 10^{-01} \cdot I + 4.52 \cdot 10^{-01} \cdot I^2 - 6.93 \cdot 10^{-04} = \frac{dI}{dy}$$

$r_0$ = 0.7, index = 4, nrun = 2: $$-1.36 \cdot 10^{-01} \cdot I - 2.51 \cdot 10^{+00} \cdot I^4 - 3.72 \cdot 10^{-04} - 2.69 \cdot 10^{+00} \cdot I^3 = \frac{dI}{dy}$$

$r_0$ = 0.7, index = 5, nrun = 1: $$-3.16 \cdot 10^{-01} \cdot I - 5.19 \cdot 10^{+00} \cdot I^4 - 1.69 \cdot 10^{+00} \cdot I^2 - 1.41 \cdot 10^{-03} - 6.74 \cdot 10^{+00} \cdot I^3 = \frac{dI}{dy}$$

$r_0$ = 0.7, index = 5, nrun = 2: $$-3.16 \cdot 10^{-01} \cdot I - 5.19 \cdot 10^{+00} \cdot I^4 - 1.69 \cdot 10^{+00} \cdot I^2 - 1.41 \cdot 10^{-03} - 6.74 \cdot 10^{+00} \cdot I^3 = \frac{dI}{dy}$$

$r_0$ = 0.8, index = 0, nrun = 0: $$-2.48 \cdot 10^{-01} \cdot I + 2.11 \cdot 10^{-01} \cdot I^2 - 1.62 \cdot 10^{-03} = \frac{dI}{dy}$$

$r_0$ = 0.8, index = 0, nrun = 1: $$-2.48 \cdot 10^{-01} \cdot I + 2.11 \cdot 10^{-01} \cdot I^2 - 1.62 \cdot 10^{-03} = \frac{dI}{dy}$$

$r_0$ = 0.8, index = 0, nrun = 2: $$-3.47 \cdot 10^{-01} \cdot I - 2.55 \cdot 10^{-03} = \frac{dI}{dy}$$

$r_0$ = 0.8, index = 1, nrun = 0: $$-3.47 \cdot 10^{-01} \cdot I - 2.55 \cdot 10^{-03} = \frac{dI}{dy}$$

$r_0$ = 0.8, index = 1, nrun = 1: $$-3.47 \cdot 10^{-01} \cdot I - 2.55 \cdot 10^{-03} = \frac{dI}{dy}$$

$r_0$ = 0.8, index = 1, nrun = 2: $$-3.47 \cdot 10^{-01} \cdot I - 2.55 \cdot 10^{-03} = \frac{dI}{dy}$$

$r_0$ = 0.8, index = 2, nrun = 0: $$-2.48 \cdot 10^{-01} \cdot I + 2.11 \cdot 10^{-01} \cdot I^2 - 1.62 \cdot 10^{-03} = \frac{dI}{dy}$$

$r_0$ = 0.8, index = 2, nrun = 1: $$-3.47 \cdot 10^{-01} \cdot I - 2.55 \cdot 10^{-03} = \frac{dI}{dy}$$

$r_0$ = 0.8, index = 2, nrun = 2: $$-3.47 \cdot 10^{-01} \cdot I - 2.55 \cdot 10^{-03} = \frac{dI}{dy}$$

$r_0$ = 0.8, index = 3, nrun = 0: $$-3.47 \cdot 10^{-01} \cdot I - 2.55 \cdot 10^{-03} = \frac{dI}{dy}$$

$r_0$ = 0.8, index = 3, nrun = 1: $$-3.47 \cdot 10^{-01} \cdot I - 2.55 \cdot 10^{-03} = \frac{dI}{dy}$$

$r_0$ = 0.8, index = 3, nrun = 2: $$-3.47 \cdot 10^{-01} \cdot I - 2.55 \cdot 10^{-03} = \frac{dI}{dy}$$

$r_0$ = 0.8, index = 4, nrun = 0: $$-2.48 \cdot 10^{-01} \cdot I + 2.11 \cdot 10^{-01} \cdot I^2 - 1.62 \cdot 10^{-03} = \frac{dI}{dy}$$

$r_0$ = 0.8, index = 4, nrun = 1: $$-3.47 \cdot 10^{-01} \cdot I - 2.55 \cdot 10^{-03} = \frac{dI}{dy}$$

$r_0$ = 0.8, index = 4, nrun = 2: $$-3.47 \cdot 10^{-01} \cdot I - 2.55 \cdot 10^{-03} = \frac{dI}{dy}$$

$r_0$ = 0.8, index = 5, nrun = 0: $$-2.48 \cdot 10^{-01} \cdot I + 2.11 \cdot 10^{-01} \cdot I^2 - 1.62 \cdot 10^{-03} = \frac{dI}{dy}$$

$r_0$ = 0.8, index = 5, nrun = 1: $$-2.48 \cdot 10^{-01} \cdot I + 2.11 \cdot 10^{-01} \cdot I^2 - 1.62 \cdot 10^{-03} = \frac{dI}{dy}$$

$r_0$ = 0.8, index = 5, nrun = 2: $$-3.47 \cdot 10^{-01} \cdot I - 2.55 \cdot 10^{-03} = \frac{dI}{dy}$$

$r_0$ = 0.9, index = 0, nrun = 0: $$-3.91 \cdot 10^{-01} \cdot I - 2.55 \cdot 10^{-03} = \frac{dI}{dy}$$

$r_0$ = 0.9, index = 0, nrun = 1: $$-5.05 \cdot 10^{-01} \cdot I - 2.03 \cdot 10^{-01} \cdot I^2 - 3.50 \cdot 10^{-03} = \frac{dI}{dy}$$

$r_0$ = 0.9, index = 0, nrun = 2: $$-5.05 \cdot 10^{-01} \cdot I - 2.03 \cdot 10^{-01} \cdot I^2 - 3.50 \cdot 10^{-03} = \frac{dI}{dy}$$

$r_0$ = 0.9, index = 1, nrun = 0: $$-3.91 \cdot 10^{-01} \cdot I - 2.55 \cdot 10^{-03} = \frac{dI}{dy}$$

$r_0$ = 0.9, index = 1, nrun = 1: $$-5.05 \cdot 10^{-01} \cdot I - 2.03 \cdot 10^{-01} \cdot I^2 - 3.50 \cdot 10^{-03} = \frac{dI}{dy}$$

$r_0$ = 0.9, index = 1, nrun = 2: $$-3.91 \cdot 10^{-01} \cdot I - 2.55 \cdot 10^{-03} = \frac{dI}{dy}$$

$r_0$ = 0.9, index = 2, nrun = 0: $$-3.91 \cdot 10^{-01} \cdot I - 2.55 \cdot 10^{-03} = \frac{dI}{dy}$$

$r_0$ = 0.9, index = 2, nrun = 1: $$-5.05 \cdot 10^{-01} \cdot I - 2.03 \cdot 10^{-01} \cdot I^2 - 3.50 \cdot 10^{-03} = \frac{dI}{dy}$$

$r_0$ = 0.9, index = 2, nrun = 2: $$-3.91 \cdot 10^{-01} \cdot I - 2.55 \cdot 10^{-03} = \frac{dI}{dy}$$

$r_0$ = 0.9, index = 3, nrun = 0: $$-5.05 \cdot 10^{-01} \cdot I - 2.03 \cdot 10^{-01} \cdot I^2 - 3.50 \cdot 10^{-03} = \frac{dI}{dy}$$

$r_0$ = 0.9, index = 3, nrun = 1: $$-3.91 \cdot 10^{-01} \cdot I - 2.55 \cdot 10^{-03} = \frac{dI}{dy}$$

$r_0$ = 0.9, index = 3, nrun = 2: $$-3.91 \cdot 10^{-01} \cdot I - 2.55 \cdot 10^{-03} = \frac{dI}{dy}$$

$r_0$ = 0.9, index = 4, nrun = 0: $$-5.05 \cdot 10^{-01} \cdot I - 2.03 \cdot 10^{-01} \cdot I^2 - 3.50 \cdot 10^{-03} = \frac{dI}{dy}$$

$r_0$ = 0.9, index = 4, nrun = 1: $$-3.91 \cdot 10^{-01} \cdot I - 2.55 \cdot 10^{-03} = \frac{dI}{dy}$$

$r_0$ = 0.9, index = 4, nrun = 2: $$-5.05 \cdot 10^{-01} \cdot I - 2.03 \cdot 10^{-01} \cdot I^2 - 3.50 \cdot 10^{-03} = \frac{dI}{dy}$$

$r_0$ = 0.9, index = 5, nrun = 0: $$-3.91 \cdot 10^{-01} \cdot I - 2.55 \cdot 10^{-03} = \frac{dI}{dy}$$

$r_0$ = 0.9, index = 5, nrun = 1: $$-5.05 \cdot 10^{-01} \cdot I - 2.03 \cdot 10^{-01} \cdot I^2 - 3.50 \cdot 10^{-03} = \frac{dI}{dy}$$

$r_0$ = 0.9, index = 5, nrun = 2: $$-6.93 \cdot 10^{-01} \cdot I + 6.02 \cdot 10^{-01} \cdot I^4 - 8.18 \cdot 10^{-01} \cdot I^2 - 4.96 \cdot 10^{-03} = \frac{dI}{dy}$$

$r_0$ = 1, index = 0, nrun = 0: $$-5.08 \cdot 10^{-01} \cdot I - 2.65 \cdot 10^{-01} \cdot I^2 - 3.86 \cdot 10^{-03} = \frac{dI}{dy}$$

$r_0$ = 1, index = 0, nrun = 1: $$-5.08 \cdot 10^{-01} \cdot I - 2.65 \cdot 10^{-01} \cdot I^2 - 3.86 \cdot 10^{-03} = \frac{dI}{dy}$$

$r_0$ = 1, index = 0, nrun = 2: $$-3.60 \cdot 10^{-01} \cdot I - 2.51 \cdot 10^{-03} = \frac{dI}{dy}$$

$r_0$ = 1, index = 1, nrun = 0: $$-3.60 \cdot 10^{-01} \cdot I - 2.51 \cdot 10^{-03} = \frac{dI}{dy}$$

$r_0$ = 1, index = 1, nrun = 1: $$-5.08 \cdot 10^{-01} \cdot I - 2.65 \cdot 10^{-01} \cdot I^2 - 3.86 \cdot 10^{-03} = \frac{dI}{dy}$$

$r_0$ = 1, index = 1, nrun = 2: $$-3.60 \cdot 10^{-01} \cdot I - 2.51 \cdot 10^{-03} = \frac{dI}{dy}$$

$r_0$ = 1, index = 2, nrun = 0: $$-5.08 \cdot 10^{-01} \cdot I - 2.65 \cdot 10^{-01} \cdot I^2 - 3.86 \cdot 10^{-03} = \frac{dI}{dy}$$

$r_0$ = 1, index = 2, nrun = 1: $$-5.08 \cdot 10^{-01} \cdot I - 2.65 \cdot 10^{-01} \cdot I^2 - 3.86 \cdot 10^{-03} = \frac{dI}{dy}$$

$r_0$ = 1, index = 2, nrun = 2: $$-5.08 \cdot 10^{-01} \cdot I - 2.65 \cdot 10^{-01} \cdot I^2 - 3.86 \cdot 10^{-03} = \frac{dI}{dy}$$

$r_0$ = 1, index = 3, nrun = 0: $$-3.60 \cdot 10^{-01} \cdot I - 2.51 \cdot 10^{-03} = \frac{dI}{dy}$$

$r_0$ = 1, index = 3, nrun = 1: $$-5.08 \cdot 10^{-01} \cdot I - 2.65 \cdot 10^{-01} \cdot I^2 - 3.86 \cdot 10^{-03} = \frac{dI}{dy}$$

$r_0$ = 1, index = 3, nrun = 2: $$-3.60 \cdot 10^{-01} \cdot I - 2.51 \cdot 10^{-03} = \frac{dI}{dy}$$

$r_0$ = 1, index = 4, nrun = 0: $$-3.60 \cdot 10^{-01} \cdot I - 2.51 \cdot 10^{-03} = \frac{dI}{dy}$$

$r_0$ = 1, index = 4, nrun = 1: $$-3.60 \cdot 10^{-01} \cdot I - 2.51 \cdot 10^{-03} = \frac{dI}{dy}$$

$r_0$ = 1, index = 4, nrun = 2: $$-3.60 \cdot 10^{-01} \cdot I - 2.51 \cdot 10^{-03} = \frac{dI}{dy}$$

$r_0$ = 1, index = 5, nrun = 0: $$-3.60 \cdot 10^{-01} \cdot I - 2.51 \cdot 10^{-03} = \frac{dI}{dy}$$

$r_0$ = 1, index = 5, nrun = 1: $$-3.60 \cdot 10^{-01} \cdot I - 2.51 \cdot 10^{-03} = \frac{dI}{dy}$$

$r_0$ = 1, index = 5, nrun = 2: $$-3.60 \cdot 10^{-01} \cdot I - 2.51 \cdot 10^{-03} = \frac{dI}{dy}$$

